theories/ITree/Events/Writer.v
@@ -1,0 +1,19 @@
+(*| Useful instructions: State |*)
+From CTree Require Import
+  Classes
+  ITree.Core.
+
+From CTree Require Export
+  Events.WriterE.
+
+From ExtLib Require Import
+  Monoid
+  Monads
+  PPair
+  Structures.MonadWriter
+  Data.Monads.WriterMonad.
+
+Import MonadNotation.
+Local Open Scope monad_scope.
+
+Definition log {S}: S -> itree (writerE S) unit := fun s => Itree.trigger (Log s).
